theories/examples/well_bracketed.v
@@ -7,6 +7,10 @@ From intensional.examples Require Import stdpp_extra tactics.
 Set Default Proof Using "Type".
 Implicit Types t : list val.
 
+(** ** Enforcing a well-bracketing protocol (Section 5.3) *)
+
+(** *** Separation logic specification *)
+
 Definition withRes_spec `{!heapG Σ} (locked: iProp Σ) (unlocked: val → iProp Σ) (withRes: val): iProp Σ :=
   ∀ P Q (f: val),
     {{{ locked ∗ P ∗
@@ -27,6 +31,8 @@ Definition bfilelib_spec `{!heapG Σ} (P0: iProp Σ) (lib: val): iProp Σ :=
     op_spec locked unlocked op
   | _ => False
   end.
+
+(** *** The trace property [bfile_trace]: "clients only use the operation after having acquired the resource and before releasing it". *)
 
 Section Trace.
 
@@ -67,6 +73,7 @@ Definition trace3 t (f: val) :=
 
 End Trace.
 
+(** *** Definition and correctness of the wrapper code *)
 
 Module Wrap.
 Section S.
@@ -180,6 +187,7 @@ Qed.
 
 End S.
 
+(** Wrapping code for an entire library *)
 Definition lib (lib_impl: val): val :=
   match lib_impl with
   | (withRes_impl, op_impl)%V =>
@@ -187,6 +195,7 @@ Definition lib (lib_impl: val): val :=
   | _ => #()
   end.
 
+(** Correctness of the library wrapper *)
 Lemma correct `{!heapG Σ} N P0 (lib_impl: val):
   bfilelib_spec P0 lib_impl -∗
   bfilelib_spec (P0 ∗ trace_is [] ∗ trace_inv N bfile_trace) (lib lib_impl).
@@ -203,9 +212,13 @@ Qed.
 
 End Wrap.
 
+(** *** Adequacy *)
+
 Definition bfilelibN := nroot .@ "bfilelib".
 Definition empty_state : state := Build_state ∅ [] ∅.
 
+(** The trace property [bfile_trace] is satisfied at every step of the execution
+    at the level of the operational semantics. *)
 Lemma wrap_bfilelib_correct (e: val → expr) (lib: val):
   (∀ `(heapG Σ), ⊢ bfilelib_spec True lib) →
   (∀ `(heapG Σ), ⊢ ∀ P lib, bfilelib_spec P lib -∗ {{{ P }}} e lib {{{ v, RET v; True }}}) →
